Large speedup via presuppositions

coq/EasyWF.v
@@ -107,68 +107,93 @@ Notation "@@[ default ] fuel =1> fuel' ; e @@" :=
   (match fuel with
      | 0 => default
      | fuel'.+1 => e
-     end).
+   end).
 
-Print le_sort.
-Fixpoint is_easy_wf_sort l c t fuel : bool :=
-  @@[false] fuel =1> fuel';
+Notation "x <-[ default ] val ; body" :=
+  (match val with
+   | Some x => body
+   | None => default
+   end) (at level 80, right associativity).
+
+Fixpoint is_easy_wf_sort fuel :=
+  @@[fun l c t => false] fuel =1> fuel';
+    fun l c t =>
     match t with
     | var x => false
     | con n s =>
-      match lookup_sort_args l n with
-      | Some c' => is_easy_wf_subst l c s c' fuel'
-      | None => false
-      end
+      c' <-[false] lookup_sort_args l n;
+      is_easy_wf_subst fuel' l c s c'
     end@@
-with is_easy_wf_subst l c s c' fuel : bool :=
-       @@[false] fuel =1> fuel';
-         match s, c' with
-         | [::], [::] => is_easy_wf_ctx l c fuel'
+with is_easy_wf_subst fuel : lang -> ctx -> subst -> ctx -> bool :=
+       @@[fun l c s c' => false] fuel =1> fuel';
+         fun l c s c' => match s, c' with
+         | [::], [::] => is_easy_wf_ctx fuel' l c
          | e::s', t::c'' =>
-           is_easy_wf_term l c e t[/s' /] fuel'
-           && is_easy_wf_subst l c s' c'' fuel'
+           is_easy_wf_term fuel' l c e t[/s' /]
+           && is_easy_wf_subst fuel' l c s' c''
          | _, _ => false
          end@@
-with is_easy_wf_term l (c : ctx) e t fuel : bool :=
-       @@[false] fuel =1> fuel';
-         match e with
+with is_easy_wf_term fuel : lang -> ctx -> exp -> exp -> bool :=
+       @@[fun l c e t => false] fuel =1> fuel';
+         fun l c e t => match e with
          | var x =>
-           match List.nth_error c x with
-           | Some t' => is_easy_wf_ctx l c fuel' && (t == t')
+           t' <-[false] List.nth_error c x;
+           (t == t') && is_easy_wf_ctx fuel' l c
              (*TODO: get this to work && is_easy_le_sort l c c t' t fuel'*)
-           | None => false
-           end
-         | con n s => false (*TODO*)
+         | con n s =>
+           c' <-[false] lookup_term_args l n;
+             t' <-[false] lookup_term_sort l n;
+             (t'[/s/] == t) && (is_easy_wf_subst fuel' l c s c')
+              
          end@@
-with is_easy_wf_ctx l c fuel : bool :=
-       @@[false] fuel =1> fuel';
-         match c with
-         | [::] => is_easy_wf_lang l fuel'
-         | t::c' =>
-           is_easy_wf_sort l c' t fuel'
-           && is_easy_wf_ctx l c' fuel'
-         end@@
-with is_easy_wf_lang l fuel : bool :=
-       @@[false] fuel =1> fuel';
-         match l with
+with is_easy_wf_ctx fuel : lang -> ctx -> bool :=
+       @@[fun l c => false] fuel =1> fuel';
+         fun l c => match c with
          | [::] => true
-         | r::l' => 
-           is_easy_wf_rule l' r fuel'
-           && is_easy_wf_lang l' fuel'
+         | t::c' =>
+           is_easy_wf_sort fuel' l c' t
+           && is_easy_wf_ctx fuel' l c'
          end@@
-with is_easy_wf_rule l r fuel : bool :=
-       @@[false] fuel =1> fuel';
-         match r with
-         | {| c |- sort } => is_easy_wf_ctx l c fuel'
-         | {| c |- t } => is_easy_wf_sort l c t fuel'
-         | {< c1 <# c2 |- t1 <# t2 } => false
-         | {< c1 <# c2 |- e1 <# e2 .: t1 <# t2 } => false
-         end@@.
-
-Definition is_easy_le_sort l (c1 c2 : ctx) t1 t2 fuel : bool :=
+with is_easy_wf_lang fuel : lang -> bool :=
+       @@[fun l => false] fuel =1> fuel';
+         fun l => match l with
+         | [::] => true
+         | r::l' => is_easy_wf_rule fuel' l' r
+                    && is_easy_wf_lang fuel' l'
+         end@@
+with is_easy_wf_rule fuel :=
+       @@[fun l r => false] fuel =1> fuel';
+         fun l r => match r with
+         | {| c |- sort } => is_easy_wf_ctx fuel' l c
+         | {| c |- t } => is_easy_wf_sort fuel' l c t
+         | {< c1 <# c2 |- t1 <# t2 } =>
+           (is_easy_le_ctx l c1 c2 fuel')
+             && (is_easy_wf_sort fuel' l c1 t1)
+             && (is_easy_wf_sort fuel' l c2 t2)
+         | {< c1 <# c2 |- e1 <# e2 .: t1 <# t2 } =>
+           (is_easy_le_sort l c1 c2 t1 t2 fuel')
+             && (is_easy_wf_term fuel' l c1 e1 t1)
+             && (is_easy_wf_term fuel' l c2 e2 t2)
+         end@@
+with is_easy_le_sort l (c1 c2 : ctx) (t1 t2 : exp) fuel : bool :=
   @@[false] fuel =1> fuel';
-    (*refl*) ((c1 == c2) && (t1 == t2) && is_easy_wf_sort l c1 t1 fuel')
-    || (* by *) (is_easy_wf_lang l fuel' && rule_in ({<c1 <# c2 |- t1 <# t2}) l)
+    (*refl*) ((c1 == c2) && (t1 == t2) && is_easy_wf_sort fuel' l c1 t1)
+    || (* by *) (is_easy_wf_lang fuel' l && rule_in ({<c1 <# c2 |- t1 <# t2}) l)
+    (*TODO: trans, subst (these are the scary cases performance-wise)*)
+    @@
+with is_easy_le_ctx l (c1 c2 : ctx) fuel : bool :=
+       @@[false] fuel =1> fuel';
+       match c1, c2 with
+       | [::],[::] => is_easy_wf_lang fuel' l
+       | t1::c1',t2::c2' => is_easy_le_sort l c1' c2' t1 t2 fuel'
+       | _, _ => false
+       end@@.
+
+
+Definition is_easy_le_term l (c1 c2 : ctx) (e1 e2 t1 t2 : exp) fuel : bool :=
+  @@[false] fuel =1> fuel';
+    (*refl*) ((c1 == c2) && (e1 == e2) && (t1 == t2) && is_easy_wf_term fuel' l c1 e1 t1)
+    || (* by *) (is_easy_wf_lang fuel' l && rule_in ({<c1 <# c2 |- e1 <# e2 .: t1 <# t2}) l)
 (*TODO: trans, subst (these are the scary cases performance-wise)*)
 @@.
 
@@ -206,16 +231,18 @@ Ltac solve_easy_wf_from_hyps :=
   by eauto.
 
 Theorem is_easy_wf_recognizes fuel
-  : (forall l, is_easy_wf_lang l fuel -> wf_lang l)
-    /\ (forall l r, is_easy_wf_rule l r fuel -> wf_rule l r)
-    /\ (forall l c, is_easy_wf_ctx l c fuel -> wf_ctx l c)
-    /\ (forall l c t, is_easy_wf_sort l c t fuel -> wf_sort l c t)
-    /\ (forall l c s c', is_easy_wf_subst l c s c' fuel -> wf_subst l c s c')
-    /\ (forall l c e t, is_easy_wf_term l c e t fuel -> wf_term l c e t).
+  : (forall l, is_easy_wf_lang fuel l -> wf_lang l)
+    /\ (forall l r, wf_lang l -> is_easy_wf_rule fuel l r -> wf_rule l r)
+    /\ (forall l c, wf_lang l -> is_easy_wf_ctx fuel l c -> wf_ctx l c)
+    /\ (forall l c t, wf_lang l -> is_easy_wf_sort fuel l c t -> wf_sort l c t)
+    /\ (forall l c s c', wf_lang l -> is_easy_wf_subst fuel l c s c' -> wf_subst l c s c')
+    /\ (forall l c e t, wf_lang l -> is_easy_wf_term fuel l c e t -> wf_term l c e t)
+    /\ (forall l c1 c2, wf_lang l -> is_easy_le_ctx l c1 c2 fuel -> le_ctx l c1 c2)
+    /\ (forall l c1 c2 t1 t2, wf_lang l -> is_easy_le_sort l c1 c2 t1 t2 fuel -> le_sort l c1 c2 t1 t2).
 Proof.
   elim: fuel => //=.
   move => fuel.
-  case => [IHlang [IHrule [IHctx [IHsort [IHsubst IHterm]]]]].
+  case => [IHlang [IHrule [IHctx [IHsort [IHsubst [IHterm [IHlectx IHlesort]]]]]]].
   split.
   1:{
     case; auto.
@@ -225,11 +252,16 @@ Proof.
   1:{
     move => l.
     case; auto.
+    move => c c0 e e0 wfl.
+    solve_easy_wf_from_hyps.
+    move => c c0 e e0 t t0 wfl.
+    solve_easy_wf_from_hyps.
   }
   split.
   1:{
     move => l.
     case; auto.
+    move => a l0 wfl.
     solve_easy_wf_from_hyps.
   }
   split.
@@ -241,6 +273,7 @@ Proof.
     case lsa: (lookup_rule 0 l n) => //=.
     case: _a_ lsa => //=.
     move => c' /lookup_rule_is_nth' => isn.
+    move => wfl.
     solve_easy_wf_from_hyps.
   }
   split.
@@ -250,37 +283,101 @@ Proof.
     case => //=; by eauto.
     move => e s.
     case => //=.
+    move => a l0 wfl.
+    solve_easy_wf_from_hyps.
+  }
+  split.
+  {
+    move => l c.
+    case => //=.
+    move => n t wfl.
+    case lne: (List.nth_error c n) =>//=.
+    repeat first [ case /andP
+                 | view_is_easy_IH_and_intro
+                 | intro ].
+    constructor; eauto.
+    move: a => /eqP -> => //.
+    unfold lookup_term_args.
+    unfold lookup_term_sort.
+    move => n s t.
+    case lsa: (lookup_rule 0 l n) => //=.
+    case: _a_ lsa => //=.
+    move => c' t' /lookup_rule_is_nth' => isn wfl.
+    case /andP.
+    move /eqP <-.
+    solve_easy_wf_from_hyps.
+  }
+  split.
+  1:{
+    move => l.
+    case => //=.
+    case => //=; auto.
+    move => t1 c1.
+    case => //.
     solve_easy_wf_from_hyps.
   }
   1:{
-    move => l c.
-    case => //=.
-    move => n t.
-    case lne: (List.nth_error c n) =>//=.
-  repeat first [ case /andP
+    intro_to is_true.
+    case /orP.
+    - case ceq:(c1 == c2) =>//=; move: ceq => /eqP ->.
+      case teq:(t1 == t2) =>//=; move: teq => /eqP ->.
+      solve_easy_wf_from_hyps.
+    - repeat first [ case /andP
           | view_is_easy_IH_and_intro
           | intro ].
-  constructor; eauto.
-  move: b => /eqP -> => //.
+      move: b => /rule_inP.
+      eauto.
   }
 Qed.
 
-Ltac get_is_easy_goal :=
+
+Theorem is_easy_le_term_recognizes fuel
+  : (forall l c1 c2 e1 e2 t1 t2,
+        wf_lang l ->
+        is_easy_le_term l c1 c2 e1 e2 t1 t2 fuel ->
+        le_term l c1 c2 e1 e2 t1 t2).
+Proof.
+  elim: fuel => //=.
+  intros until t2.
+  move => wfl.
+  case /orP.
+  {
+    case ceq: (c1 == c2) => //=; move: ceq => /eqP ->.
+    case eeq: (e1 == e2) => //=; move: eeq => /eqP ->.
+    case teq: (t1 == t2) => //=; move: teq => /eqP ->.
+    move => et.
+    eapply is_easy_wf_recognizes in et.
+    all: eauto.
+  }
+  {
+    case /andP.
+    move => et.
+    eapply is_easy_wf_recognizes in et.
+    move /rule_inP.
+    eauto.
+  }
+Qed.
+
+
+Ltac get_is_easy_goal n :=
   match goal with
-  | |- wf_lang ?L => type_term (is_easy_wf_lang L)
-  | |- wf_rule ?L ?r => type_term (is_easy_wf_rule L r)
-  | |- wf_ctx ?L ?c => type_term (is_easy_wf_ctx L c)
-  | |- wf_sort ?L ?c ?t => type_term (is_easy_wf_sort L c t)
-  | |- wf_term ?L ?c ?e ?t => type_term (is_easy_wf_term L c e t)
-  | |- wf_subst ?L ?c ?s ?c' => type_term (is_easy_wf_subst L c s c')
+  | |- wf_lang ?L => type_term (is_easy_wf_lang n L)
+  | |- wf_rule ?L ?r => type_term (is_easy_wf_rule n L r)
+  | |- wf_ctx ?L ?c => type_term (is_easy_wf_ctx n L c)
+  | |- wf_sort ?L ?c ?t => type_term (is_easy_wf_sort n L c t)
+  | |- wf_term ?L ?c ?e ?t => type_term (is_easy_wf_term n L c e t)
+  | |- wf_subst ?L ?c ?s ?c' => type_term (is_easy_wf_subst n L c s c')
+  | |- le_sort ?l ?c1 ?c2 ?t1 ?t2 => type_term (is_easy_le_sort n l c1 c2 t1 t2)
+  | |- le_term ?l ?c1 ?c2 ?e1 ?e2 ?t1 ?t2 => type_term (is_easy_le_term n l c1 c2 e1 e2 t1 t2)
   end.
 
 (* Tactics for using the partial recognizer to prove a language well-formed *)
 (*TODO: generalize to all constructs, not just langs*)
 Ltac solve_easy_wf n :=
-  let easy_goal := get_is_easy_goal in
-  suff: easy_goal n;
-  [ intros; eapply is_easy_wf_recognizes; by eauto
+  let easy_goal := get_is_easy_goal n in
+  suff: easy_goal;
+  [ intros; first [ eapply is_easy_wf_recognizes
+                  | eapply is_easy_le_term_recognizes]; by eauto
   | by compute].
 
 Tactic Notation "solve_easy_wf" constr(n) := solve_easy_wf n.
